Computability/Constructions/archive.lean
@@ -1,3 +1,7 @@
+import Computability.Constructions.Basic
+
+open Nat.RecursiveIn.Code
+
 -- section bfind
 -- namespace Nat.RecursiveIn.Code
 -- def p_bfind (O) (cf) (b) (n) := n≤b ∧ eval_prim O cf n = 0
@@ -30,3 +34,216 @@
 -- @[simp] theorem c_bfind_ev : eval O c_bfind (Nat.pair lN i) = o2n (n2l lN)[i]? := by simp [← eval_prim_eq_eval c_bfind_ev_pr]
 -- end Nat.RecursiveIn.Code
 -- end bfind
+
+
+
+section l_append
+def Nat.list_append (list index:ℕ):ℕ:=Nat.pair (list.l+1) $ Nat.pair list.r index
+namespace Nat.RecursiveIn.Code
+def c_l_append := pair (succ.comp $ left.comp left) (pair (right.comp left) right)
+@[simp] theorem c_l_append_ev_pr:code_prim c_l_append := by unfold c_l_append; repeat (first|assumption|simp|constructor)
+@[simp] theorem c_l_append_evp:eval_prim O c_l_append = unpaired2 Nat.list_append := by unfold Nat.list_append; simp [c_l_append,eval_prim];
+@[simp] theorem c_l_append_ev:eval O c_l_append = unpaired2 Nat.list_append := by rw [← eval_prim_eq_eval c_l_append_ev_pr]; simp only [c_l_append_evp]
+end Nat.RecursiveIn.Code
+-- theorem Nat.PrimrecIn.l_append:Nat.PrimrecIn O Nat.l_append := by ...
+-- theorem Nat.Primrec.l_append:Nat.Primrec Nat.l_append := by ...
+end l_append
+
+section l_get_last
+def Nat.list_get_last_aux (list index:ℕ):ℕ:=
+  match index with
+  | 0 => list.r
+  | Nat.succ prev_index => (Nat.list_get_last_aux list prev_index).l
+def Nat.list_get_lastn (list index:ℕ):ℕ:=(Nat.list_get_last_aux list index).r
+def Nat.list_get_last (list:ℕ) :=list.r.r
+def Nat.list_size (list:ℕ) := list.l
+def Nat.list_get (list index:ℕ) := Nat.list_get_lastn list (list.list_size-1-index)
+
+#check (Nat.pair 2 (Nat.pair (Nat.pair 0 132) 42))
+#eval Nat.list_get_last (Nat.pair 2 (Nat.pair (Nat.pair 0 132) 42))
+#eval Nat.list_get_lastn (Nat.pair 2 (Nat.pair (Nat.pair 0 132) 42)) 0
+#eval Nat.list_get_lastn (Nat.pair 2 (Nat.pair (Nat.pair 0 132) 42)) 1
+
+namespace Nat.RecursiveIn.Code
+def c_l_get_lastn_aux := prec right (left.comp $ right.comp right)
+@[simp] theorem c_l_get_lastn_aux_ev_pr:code_prim c_l_get_lastn_aux := by unfold c_l_get_lastn_aux; repeat (first|assumption|simp|constructor)
+@[simp] theorem c_l_get_lastn_aux_evp:eval_prim O c_l_get_lastn_aux = unpaired2 Nat.list_get_last_aux := by
+  simp [c_l_get_lastn_aux,eval_prim];
+  funext n;
+  simp [unpaired2]
+  induction n.r with
+  | zero => exact rfl
+  | succ n h => exact congrArg Prod.fst (congrArg unpair h)
+@[simp] theorem c_l_get_lastn_aux_ev:eval O c_l_get_lastn_aux = unpaired2 Nat.list_get_last_aux := by rw [← eval_prim_eq_eval c_l_get_lastn_aux_ev_pr]; simp only [c_l_get_lastn_aux_evp];
+
+def c_l_get_lastn := right.comp c_l_get_lastn_aux
+@[simp] theorem c_l_get_lastn_ev_pr:code_prim c_l_get_lastn := by unfold c_l_get_lastn; repeat (first|assumption|simp|constructor)
+@[simp] theorem c_l_get_lastn_evp:eval_prim O c_l_get_lastn = unpaired2 Nat.list_get_lastn := by
+  unfold list_get_lastn
+  simp [c_l_get_lastn,eval_prim];
+@[simp] theorem c_l_get_lastn_ev:eval O c_l_get_lastn = unpaired2 Nat.list_get_lastn := by rw [← eval_prim_eq_eval c_l_get_lastn_ev_pr]; simp only [c_l_get_lastn_evp];
+
+def c_l_get_last := c_l_get_lastn.comp₂ c_id (c_const 0)
+@[simp] theorem c_l_get_last_ev_pr:code_prim c_l_get_last := by unfold c_l_get_last; repeat (first|assumption|simp|constructor);
+@[simp] theorem c_l_get_last_evp:eval_prim O c_l_get_last = Nat.list_get_last := by
+  unfold list_get_last
+  simp [c_l_get_last,eval_prim];
+  exact rfl
+@[simp] theorem c_l_get_last_ev:eval O c_l_get_last = Nat.list_get_last := by rw [← eval_prim_eq_eval c_l_get_last_ev_pr]; simp only [c_l_get_last_evp];
+end Nat.RecursiveIn.Code
+-- theorem Nat.PrimrecIn.l_get:Nat.PrimrecIn O Nat.l_get := by ...
+-- theorem Nat.Primrec.l_get:Nat.Primrec Nat.l_get := by ...
+end l_get_last
+
+
+-- takes a pair (list,index)
+section l_get
+namespace Nat.RecursiveIn.Code
+def c_l_get := c_l_get_lastn.comp₂ left (c_sub.comp₂ (c_pred.comp (left.comp left)) (right))
+@[simp] theorem c_l_get_ev_pr:code_prim c_l_get := by unfold c_l_get; repeat (first|assumption|simp|constructor)
+@[simp] theorem c_l_get_evp:eval_prim O c_l_get = unpaired2 Nat.list_get := by
+  unfold Nat.list_get;
+  simp [c_l_get,eval_prim];
+  funext xs
+  exact rfl
+@[simp] theorem c_l_get_ev:eval O c_l_get = unpaired2 Nat.list_get := by rw [← eval_prim_eq_eval c_l_get_ev_pr]; simp only [c_l_get_evp]
+end Nat.RecursiveIn.Code
+-- theorem Nat.PrimrecIn.l_get:Nat.PrimrecIn O Nat.l_get := by ...
+-- theorem Nat.Primrec.l_get:Nat.Primrec Nat.l_get := by ...
+end l_get
+
+-- takes a pair (list,index). returns l[i]+1 if exists, 0 otherwise
+section l_get_opt
+namespace Nat.RecursiveIn.Code
+def c_l_get_opt :=
+  let list        := left
+  let list_length := left.comp list
+  let index       := right
+
+  c_if_lt_te.comp₄ index list_length
+  (succ.comp $ c_l_get.comp₂ list index)
+  (c_const 0)
+  -- c_l_get_opt_lastn.comp₂ left (c_sub.comp₂ (c_pred.comp (left.comp left)) (right))
+@[simp] theorem c_l_get_opt_ev_pr:code_prim c_l_get_opt := by unfold c_l_get_opt; repeat (first|assumption|simp|constructor)
+@[simp] theorem c_l_get_opt_evp {O list index}:eval_prim O c_l_get_opt (Nat.pair list index) = if index<Nat.list_size list then (Nat.list_get list index)+1 else 0 := by
+  simp [c_l_get_opt,eval_prim, comp₄];
+  exact rfl
+-- @[simp] theorem c_l_get_opt_ev:eval O c_l_get_opt = unpaired2 Nat.list_get := by rw [← eval_prim_eq_eval c_l_get_opt_ev_pr]; simp only [c_l_get_opt_evp]
+end Nat.RecursiveIn.Code
+-- theorem Nat.PrimrecIn.l_get_opt:Nat.PrimrecIn O Nat.l_get_opt := by ...
+-- theorem Nat.Primrec.l_get_opt:Nat.Primrec Nat.l_get_opt := by ...
+end l_get_opt
+
+
+@[simp] theorem Nat.list_get_last_append : Nat.list_get_last (Nat.list_append lst x) = x := by
+  unfold list_append
+  unfold list_get_last
+  simp
+
+
+
+section efl
+namespace Nat.RecursiveIn.Code
+def c_efl:ℕ→ℕ:=fun c=>c_l_append.comp (pair c_id c)
+-- def c_efl:=fun c=>c_l_append.comp₂ c_id c
+@[simp] theorem c_efl_ev_pr (h:code_prim c):code_prim $ c_efl c := by unfold c_efl; repeat (first|assumption|simp|constructor)
+
+-- @[simp] theorem c_efl_pr_aux:Primrec (pair c_id) := by
+--   refine Primrec.projection ?_
+--   apply PrimrecIn.PrimrecIn₂_iff_Primrec₂.mp
+--   intro O
+--   apply pair_prim
+-- @[simp] theorem c_efl_pr: Nat.Primrec c_efl := by
+--   refine Primrec.nat_iff.mp ?_
+--   apply c_efl_pr_aux
+
+-- huh interesting, it doesn't care about c being code_prim or not.
+@[simp] theorem c_efl_evp:eval_prim O (c_efl c) x= Nat.list_append x (eval_prim O c x) := by
+  unfold list_append
+  simp [c_efl,eval_prim];
+  unfold list_append
+  simp
+@[simp] theorem c_efl_ev : eval O (c_efl c) x = Nat.list_append <$> x <*> (eval O c x) := by
+  unfold Nat.list_append
+  simp [c_efl,eval]
+  simp [Seq.seq]
+
+  exact Part.bind_some_eq_map x.list_append (eval O c x)
+  -- exact Part.bind_some_eq_map x.list_append (eval O (decodeCode c) x)
+end Nat.RecursiveIn.Code
+-- theorem Nat.PrimrecIn.efl:Nat.PrimrecIn O Nat.efl := by ...
+-- theorem Nat.Primrec.efl:Nat.Primrec Nat.efl := by ...
+-- theorem c_efl_ev_left (h:(eval O c x).Dom) : eval O (left.comp $ c_efl c) x = x := by
+--   have h0 : (eval O c x).get h ∈ (eval O c x) := by exact Part.get_mem h
+--   have h1 : eval O c x = Part.some ((eval O c x).get h) := by exact Part.get_eq_iff_eq_some.mp rfl
+
+--   simp [c_efl, eval]
+--   rw [h1]
+--   -- should maybe define some theorem that simplfies the Nat.pair <*> business
+--   simp [Seq.seq]
+--   exact Part.Dom.bind h fun y ↦ Part.some x
+end efl
+
+@[simp] theorem last_efl : eval_prim O (c_l_get_last.comp (c_efl c)) = eval_prim O c := by
+  simp only [eval_prim]
+  simp
+
+
+
+
+def Nat.list_empty := Nat.pair 0 0
+def Nat.list_singleton (ele:ℕ) := Nat.list_append Nat.list_empty ele
+namespace Nat.RecursiveIn.Code
+def c_list_singleton (ele:Code): Code := c_l_append.comp₂ Nat.list_empty ele
+end Nat.RecursiveIn.Code
+
+open Nat in
+@[simp] theorem append_empty : (list_empty.list_append x).list_get 0 = x := by
+  unfold list_empty
+  unfold list_append
+  unfold list_get
+  unfold list_get_lastn
+  unfold list_get_last_aux
+  unfold list_size
+  simp
+
+
+open Nat in
+@[simp] theorem append_get_last_aux {l:ℕ}: l.list_get_last_aux i =  (l.list_append x).list_get_last_aux (i+1) := by
+  induction i
+  ·
+    unfold list_get_last_aux
+    unfold list_get_last_aux
+    unfold list_append
+    simp
+  · expose_names
+    unfold list_append
+    unfold list_get_last_aux
+    rw [h]
+    unfold list_append
+    simp
+
+open Nat in
+@[simp] theorem append_getlastn {l:ℕ}: l.list_get_lastn i = (l.list_append x).list_get_lastn (i+1) := by
+  unfold list_get_lastn
+  rw [append_get_last_aux]
+
+open Nat in
+@[simp] theorem append_size {l:ℕ} : (l.list_append x).list_size = l.list_size +1 := by
+  unfold list_append
+  unfold list_size
+  simp
+
+open Nat in
+@[simp] theorem append_get {l:ℕ} (hi:i<l.list_size): l.list_get i = (l.list_append x).list_get i := by
+  unfold list_get
+  simp only [append_size]
+  simp
+  have hi5 : l.list_size - i - 1 = l.list_size - 1 - i := by exact Simproc.sub_add_eq_comm l.list_size i 1
+  have hi6 : l.list_size - i > 0 := by exact zero_lt_sub_of_lt hi
+  have main_rewrite : (l.list_size - 1 - i)+1 = l.list_size - i := by
+    rw [←hi5]
+    exact Nat.sub_add_cancel hi6
+
+  rw [←main_rewrite]
+  exact append_getlastn
