Computability/Constructions/CovRec.lean
@@ -1,4 +1,5 @@
 import Computability.Constructions.Basic
+import Computability.Constructions.List
 open Nat.RecursiveIn.Code
 
 section l_append
